theories/Labelled_Transition_System/Examples_of_LTS/ACCS/ACCSInstance.v
@@ -23,7 +23,17 @@
    SOFTWARE.
 *)
 
-From Stdlib.Program Require Import Equality.
+From TestingTheory Require Import VACCS_Instance.
+
+Module Type ACCS.
+
+  Include VACCS_lts.
+
+  Axiom Value_is_unit : Value = unit.
+
+End ACCS.
+
+(* From Stdlib.Program Require Import Equality.
 From Stdlib.Strings Require Import String.
 From Stdlib Require Import Relations.
 From Stdlib.Wellfounded Require Import Inverse_Image.
@@ -32,9 +42,9 @@ From stdpp Require Import base countable finite gmap list gmultiset strings.
 From TestingTheory Require Import InListPropHelper InputOutputActions ActTau OldTransitionSystems Must 
       Completeness Soundness DefinitionCI Normalisation MultisetLTSConstruction
       GeneralizeLtsOutputs ForwarderConstruction ParallelLTSConstruction Testing_Predicate
-      (* gLts *) (* Bisimulation *).
+      (* gLts *) (* Bisimulation *). *)
 
-
+(*
 (** *** ACCS properties *)
 Definition name := string.
 Definition name_eq_dec : forall (x y : name), { x = y } + { x <> y } := string_dec.
@@ -1422,4 +1432,6 @@ Proof.
     eapply elem_of_union. left. now eapply gmultiset_elem_of_dom.
     eapply elem_of_union. right. now eapply gmultiset_elem_of_dom.
 Qed.
+*)
+
 *)
