theories/Labelled_Transition_System/Examples_of_LTS/CCS/CCS_Must_Characterization.v
@@ -26,19 +26,25 @@
 
 From Stdlib.Program Require Import Equality.
 From Stdlib.Strings Require Import String.
-From stdpp Require Import base countable finite gmap list gmultiset strings.
 From Stdlib Require Import Relations.
 From Stdlib.Wellfounded Require Import Inverse_Image.
-From TestingTheory Require Import VCCS_Must_Characterization.
+
+From stdpp Require Import base countable finite gmap list gmultiset strings.
+From TestingTheory Require Import InListPropHelper InputOutputActions ActTau Must 
+      Completeness Soundness Equivalence  DefinitionAS MultisetLTSConstruction
+      GeneralizeLtsOutputs ForwarderConstruction ParallelLTSConstruction InteractionBetweenLts  Testing_Predicate
+      gLts Bisimulation Lts_OBA Lts_FW Lts_OBA_FB GeneralizeLtsOutputs
+      MultisetLTSConstruction Lts_Finite_Output_Chain.
+From TestingTheory Require Import MustE FiniteImageLTS VCCS_Must_Characterization.
 
 Module Type CCS_Must_Alt_Corollary.
 Include VCCS_Must_Alt_Corollary.
 
 Axiom Value_is_unit : Value = unit.
 
-Corollary bhv_iff_ctx_CCS (p q : proc) : p ⊑ₘᵤₛₜᵢ q <-> p ≼ₐₛ q.
+Corollary bhv_iff_ctx_CCS (p q : proc) : p ⊑ₘᵤₛₜᵢ q <-> p ▷ ∅ ≼ₐₛ q ▷ ∅.
 Proof.
-  (* eapply bhv_iff_ctx_VCCS. *) admit.
-Admitted.
+   eapply bhv_iff_ctx_VCCS.
+Qed.
 
 End CCS_Must_Alt_Corollary.
