theories/Labelled_Transition_System/Examples_of_LTS/VACCS/VACCS_Must_Characterization.v
@@ -2,35 +2,35 @@ From stdpp Require Import gmap gmultiset.
 From Stdlib.Program Require Import Equality.
 From Stdlib.Wellfounded Require Import Inverse_Image.
 From TestingTheory Require Import InputOutputActions OldTransitionSystems ActTau .
-From TestingTheory Require Export VACCS VACCS.Congruence VACCS_Instance
-  VACCS_ta VACCS_tc DefinitionAS Must ForwarderConstruction ParallelLTSConstruction
+From TestingTheory Require Import
+  VACCS_ta_tc_gen DefinitionAS Must ForwarderConstruction ParallelLTSConstruction
   InteractionBetweenLts GeneralizeLtsOutputs Completeness Equivalence Soundness
   Testing_Predicate Bisimulation Lts_OBA.
 
+
+Module Type VACCS_Must_Alt_Corollary.
+Include VACCS_ta_tc.
 
 Corollary bhv_iff_ctx_VACCS (p q : proc) : p ⊑ₘᵤₛₜᵢ q <-> p ▷ ∅ ≼ₐₛ q ▷ ∅.
 Proof.
   split.
   - intro Hyp. eapply @equivalence_acc_set_and_must_i; eauto.
 
-
-
     exact VACCS_gLtsFiniteImage. exact VACCS_gLtsFiniteImage. exact VACCS_gLtsFiniteImage.
-    exact Interaction_between_FW_ACCS_and_ACCS. exact Interaction_between_FW_ACCS_and_ACCS.
-    exact (@gAbsAction (ExtAct TypeOfActions)).
-    (* exact (gen_conv_gen_spec_conv_inst _)*) admit.
-    (* exact gen_acc_gen_spec_acc_inst. *) admit.
-    exact VACCS_gLtsOBAFB. exact VACCS_FiniteOutputChains.
+    exact Interaction_between_FW_VACCS_and_VACCS. exact Interaction_between_FW_VACCS_and_VACCS.
+    (* exact gen_conv_gen_spec_conv_inst. *) admit.
+    (* exact gen_acc_gen_spec_acc_inst.*) admit.
+    exact VACCS_gLtsOBAFB. exact VACCS_gFiniteOutputChain_LtsOba.
 
 
   - intro Hyp. eapply @equivalence_acc_set_and_must_i in Hyp; eauto.
 
     exact VACCS_gLtsFiniteImage. exact VACCS_gLtsFiniteImage. exact VACCS_gLtsFiniteImage.
-    exact Interaction_between_FW_ACCS_and_ACCS. exact Interaction_between_FW_ACCS_and_ACCS.
-    exact (@gAbsAction (ExtAct TypeOfActions)).
-    (* exact (gen_conv_gen_spec_conv_inst _)*) admit.
-    (* exact gen_acc_gen_spec_acc_inst. *) admit.
-    exact VACCS_gLtsOBAFB. exact VACCS_FiniteOutputChains.
+    exact Interaction_between_FW_VACCS_and_VACCS. exact Interaction_between_FW_VACCS_and_VACCS.
+    exact FinitaryAbsVACCS. exact FinitaryAbsVACCS.
+    (* exact gen_conv_gen_spec_conv_inst. *) admit.
+    (* exact gen_acc_gen_spec_acc_inst.*) admit.
+    exact VACCS_gLtsOBAFB. exact VACCS_gFiniteOutputChain_LtsOba.
 Admitted.
 
-
+End VACCS_Must_Alt_Corollary.
